examples/TensorSquare.mo
@@ -1,0 +1,8 @@
+model TensorSquare
+  input Real u[2];
+  output Real x[2](each start=0, each fixed=true);
+  output Real J[2,2];
+equation
+  der(x) = u .* u;
+  J = jacobian (u .* u, u);
+end TensorSquare;
